bitvector, var_value proved

tests/bitvector1/bitvector1_TestDoubleOfInt_exp_const_1.v
@@ -266,8 +266,8 @@ Axiom to_nat_of_zero : forall (b:bv) (i:Z) (j:Z), ((i <= j)%Z /\
   (0%Z <= i)%Z) -> ((forall (k:Z), ((k <= j)%Z /\ (i <= k)%Z) -> ((nth b
   k) = false)) -> ((to_nat_sub b j i) = 0%Z)).
 
-Axiom to_nat_of_one : forall (b:bv) (i:Z) (j:Z), ((j <= i)%Z /\
-  (0%Z <= j)%Z) -> ((forall (k:Z), ((k <= j)%Z /\ (i <= k)%Z) -> ((nth b
+Axiom to_nat_of_one : forall (b:bv) (i:Z) (j:Z), ((i <= j)%Z /\
+  (0%Z <= i)%Z) -> ((forall (k:Z), ((k <= j)%Z /\ (i <= k)%Z) -> ((nth b
   k) = true)) -> ((to_nat_sub b j
   i) = ((pow2 ((j - i)%Z + 1%Z)%Z) - 1%Z)%Z)).
 
@@ -443,8 +443,8 @@ Axiom to_nat_of_zero1 : forall (b:bv1) (i:Z) (j:Z), ((i <= j)%Z /\
   (0%Z <= i)%Z) -> ((forall (k:Z), ((k <= j)%Z /\ (i <= k)%Z) -> ((nth1 b
   k) = false)) -> ((to_nat_sub1 b j i) = 0%Z)).
 
-Axiom to_nat_of_one1 : forall (b:bv1) (i:Z) (j:Z), ((j <= i)%Z /\
-  (0%Z <= j)%Z) -> ((forall (k:Z), ((k <= j)%Z /\ (i <= k)%Z) -> ((nth1 b
+Axiom to_nat_of_one1 : forall (b:bv1) (i:Z) (j:Z), ((i <= j)%Z /\
+  (0%Z <= i)%Z) -> ((forall (k:Z), ((k <= j)%Z /\ (i <= k)%Z) -> ((nth1 b
   k) = true)) -> ((to_nat_sub1 b j
   i) = ((pow2 ((j - i)%Z + 1%Z)%Z) - 1%Z)%Z)).
 
@@ -533,95 +533,77 @@ Axiom double_of_bv64_value : forall (b:bv1), ((0%Z <  (to_nat_sub1 b 62%Z
   62%Z 52%Z) - 1023%Z)%Z))%R * (1%R + ((IZR (to_nat_sub1 b 51%Z
   0%Z)) * (pow21 (-52%Z)%Z))%R)%R)%R).
 
+Axiom nth_const1 : forall (i:Z), ((0%Z <= i)%Z /\ (i <= 30%Z)%Z) ->
+  ((nth1 (concat (from_int 1127219200%Z) (from_int 2147483648%Z))
+  i) = false).
+
+Axiom nth_const2 : ((nth1 (concat (from_int 1127219200%Z)
+  (from_int 2147483648%Z)) 31%Z) = true).
+
+Axiom nth_const3 : forall (i:Z), ((32%Z <= i)%Z /\ (i <= 51%Z)%Z) ->
+  ((nth1 (concat (from_int 1127219200%Z) (from_int 2147483648%Z))
+  i) = false).
+
+Axiom nth_const4 : forall (i:Z), ((52%Z <= i)%Z /\ (i <= 53%Z)%Z) ->
+  ((nth1 (concat (from_int 1127219200%Z) (from_int 2147483648%Z)) i) = true).
+
+Axiom nth_const5 : forall (i:Z), ((54%Z <= i)%Z /\ (i <= 55%Z)%Z) ->
+  ((nth1 (concat (from_int 1127219200%Z) (from_int 2147483648%Z))
+  i) = false).
+
+Axiom nth_const6 : forall (i:Z), ((56%Z <= i)%Z /\ (i <= 57%Z)%Z) ->
+  ((nth1 (concat (from_int 1127219200%Z) (from_int 2147483648%Z)) i) = true).
+
+Axiom nth_const7 : forall (i:Z), ((58%Z <= i)%Z /\ (i <= 61%Z)%Z) ->
+  ((nth1 (concat (from_int 1127219200%Z) (from_int 2147483648%Z))
+  i) = false).
+
+Axiom nth_const8 : ((nth1 (concat (from_int 1127219200%Z)
+  (from_int 2147483648%Z)) 62%Z) = true).
+
+Axiom nth_const9 : ((nth1 (concat (from_int 1127219200%Z)
+  (from_int 2147483648%Z)) 63%Z) = false).
+
 Axiom sign_const : ((nth1 (concat (from_int 1127219200%Z)
   (from_int 2147483648%Z)) 63%Z) = false).
 
-Axiom exp_const : ((to_nat_sub1 (concat (from_int 1127219200%Z)
-  (from_int 2147483648%Z)) 62%Z 52%Z) = 1075%Z).
-
-Axiom mantissa_const_nth : forall (i:Z), ((0%Z <= i)%Z /\ (i <= 30%Z)%Z) ->
-  ((nth1 (concat (from_int 1127219200%Z) (from_int 2147483648%Z))
-  i) = false).
-
-Axiom mantissa_const_31th : ((nth1 (concat (from_int 1127219200%Z)
-  (from_int 2147483648%Z)) 31%Z) = true).
-
-Axiom to_nat_mantissa_1 : ((to_nat_sub1 (concat (from_int 1127219200%Z)
-  (from_int 2147483648%Z)) 30%Z 0%Z) = 0%Z).
-
-Axiom mantissa_const_nth2 : forall (i:Z), ((32%Z <= i)%Z /\ (i <= 51%Z)%Z) ->
-  ((nth1 (concat (from_int 1127219200%Z) (from_int 2147483648%Z))
-  i) = false).
-
-Axiom mantissa_const_to_nat51 : ((to_nat_sub1 (concat (from_int 1127219200%Z)
-  (from_int 2147483648%Z)) 51%Z
-  0%Z) = (to_nat_sub1 (concat (from_int 1127219200%Z)
-  (from_int 2147483648%Z)) 31%Z 0%Z)).
-
-Axiom mantissa_const : ((to_nat_sub1 (concat (from_int 1127219200%Z)
-  (from_int 2147483648%Z)) 51%Z 0%Z) = (pow2 31%Z)).
-
-Axiom real1075m1023 : ((IZR (1075%Z - 1023%Z)%Z) = 52%R).
-
-Axiom real1075m1023_2 : ((1075%R - 1023%R)%R = 52%R).
-
-Axiom real52_a_m52 : ((((pow21 (1075%Z - 1023%Z)%Z) * (pow21 31%Z))%R * (pow21 (-52%Z)%Z))%R = (pow21 31%Z)).
-
-Axiom const_value0 : ((double_of_bv64 (concat (from_int 1127219200%Z)
-  (from_int 2147483648%Z))) = ((1%R * (pow21 (1075%Z - 1023%Z)%Z))%R * (1%R + ((pow21 31%Z) * (pow21 (-52%Z)%Z))%R)%R)%R).
-
-Axiom const_value : ((double_of_bv64 (concat (from_int 1127219200%Z)
-  (from_int 2147483648%Z))) = ((pow21 52%Z) + (pow21 31%Z))%R).
-
-Definition jpxor(i:Z): bv := (bw_xor (from_int 2147483648%Z) (from_int i)).
-
-Definition var(i:Z): bv1 := (concat (from_int 1127219200%Z) (jpxor i)).
-
-Axiom nth30_0 : forall (x:bv) (j:Z), ((0%Z <= j)%Z /\ (j <  31%Z)%Z) ->
-  ((nth (bw_xor (from_int 2147483648%Z) x) j) = (nth x j)).
-
-Axiom nth30_0_var : forall (x:Z) (j:Z), ((0%Z <= j)%Z /\ (j <  31%Z)%Z) ->
-  ((nth1 (var x) j) = (nth (from_int x) j)).
-
-Axiom nth31_var : forall (x:Z), ((nth1 (var x)
-  31%Z) = (negb (nth (from_int x) 31%Z))).
-
-Axiom nth63_32_var : forall (x:Z) (k:Z), ((32%Z <= k)%Z /\ (k <= 63%Z)%Z) ->
-  ((nth1 (var x) k) = (nth (from_int 1127219200%Z) (k - 32%Z)%Z)).
-
-Axiom sign_var : forall (x:Z), ((nth1 (var x) 63%Z) = false).
-
-Axiom exp_var : forall (x:Z), ((to_nat_sub1 (var x) 62%Z 52%Z) = 1075%Z).
-
-Axiom mantissa_var_0_30 : forall (x:Z), ((nth (from_int x) 31%Z) = false) ->
-  ((to_nat_sub1 (var x) 30%Z 0%Z) = x).
-
-Axiom mantissa_var_0_30_1 : forall (x:Z), ((nth (from_int x) 31%Z) = true) ->
-  ((to_nat_sub1 (var x) 30%Z 0%Z) = (-x)%Z).
-
-Axiom mantissa_var : forall (x:Z), ((to_nat_sub1 (var x) 51%Z
-  0%Z) = ((pow2 31%Z) + x)%Z).
-
-Definition var_as_double(x:Z): R := (double_of_bv64 (var x)).
-
 (* YOU MAY EDIT THE CONTEXT BELOW *)
-
+Open Scope Z_scope.
 (* DO NOT EDIT BELOW *)
 
-Theorem var_value0 : forall (x:Z),
-  ((var_as_double x) = ((pow21 (1075%Z - 1023%Z)%Z) * (1%R + ((IZR ((pow2 31%Z) + x)%Z) * (pow21 (-52%Z)%Z))%R)%R)%R).
+Theorem exp_const : ((to_nat_sub1 (concat (from_int 1127219200%Z)
+  (from_int 2147483648%Z)) 62%Z 52%Z) = 1075%Z).
 (* YOU MAY EDIT THE PROOF BELOW *)
-intro.
-unfold var_as_double.
-rewrite double_of_bv64_value.
-rewrite sign_var.
-rewrite sign_value_false.
-rewrite exp_var.
-rewrite mantissa_var.
-rewrite Rmult_1_l.
-auto with *.
-rewrite exp_var.
-auto with *.
+rewrite to_nat_sub_one1; auto with zarith.
+  2: apply nth_const8.
+replace (62 - 52) with 10 by omega.
+ rewrite pow2_10.
+rewrite to_nat_sub_zero1; auto with zarith.
+  2: apply nth_const7; auto with zarith.
+rewrite to_nat_sub_zero1; auto with zarith.
+  2: apply nth_const7; auto with zarith.
+rewrite to_nat_sub_zero1; auto with zarith.
+  2: apply nth_const7; auto with zarith.
+rewrite to_nat_sub_zero1; auto with zarith.
+  2: apply nth_const7; auto with zarith.
+rewrite to_nat_sub_one1; auto with zarith.
+  2: apply nth_const6; auto with zarith.
+replace (62 - 1 - 1 - 1 - 1 - 1 - 52) with 5 by omega.
+ rewrite pow2_5.
+rewrite to_nat_sub_one1; auto with zarith.
+  2: apply nth_const6; auto with zarith.
+replace (62 - 1 - 1 - 1 - 1 - 1 - 1 -  52) with 4 by omega.
+ rewrite pow2_4.
+rewrite to_nat_sub_zero1; auto with zarith.
+  2: apply nth_const5; auto with zarith.
+rewrite to_nat_sub_zero1; auto with zarith.
+  2: apply nth_const5; auto with zarith.
+rewrite to_nat_of_one1; auto with zarith.
+replace (62 - 1 - 1 - 1 - 1 - 1 - 1 - 1 - 1 - 1 - 52) with 1 by omega.
+replace (1+1) with 2 by omega.
+ rewrite pow2_2; auto.
+intros.
+apply nth_const4; auto with zarith.
 Qed.
 (* DO NOT EDIT BELOW *)
 
