tests/bitvector1/bitvector1_TestDoubleOfInt_var_value4_2.v
@@ -604,23 +604,28 @@ Axiom mantissa_var : forall (x:Z), ((to_nat_sub1 (var x) 51%Z
 
 Definition var_as_double(x:Z): R := (double_of_bv64 (var x)).
 
+Axiom var_value0 : forall (x:Z),
+  ((var_as_double x) = ((pow21 (1075%Z - 1023%Z)%Z) * (1%R + ((IZR ((pow2 31%Z) + x)%Z) * (pow21 (-52%Z)%Z))%R)%R)%R).
+
+Axiom from_int_sum : forall (x:Z),
+  ((IZR ((pow2 31%Z) + x)%Z) = ((IZR (pow2 31%Z)) + (IZR x))%R).
+
+Axiom var_value3 : forall (x:Z),
+  ((var_as_double x) = ((pow21 52%Z) + (((pow21 52%Z) * ((IZR (pow2 31%Z)) + (IZR x))%R)%R * (pow21 (-52%Z)%Z))%R)%R).
+
+Axiom distr_pow52 : forall (x:R),
+  ((((pow21 52%Z) * x)%R * (pow21 (-52%Z)%Z))%R = x).
+
 (* YOU MAY EDIT THE CONTEXT BELOW *)
 
 (* DO NOT EDIT BELOW *)
 
-Theorem var_value0 : forall (x:Z),
-  ((var_as_double x) = ((pow21 (1075%Z - 1023%Z)%Z) * (1%R + ((IZR ((pow2 31%Z) + x)%Z) * (pow21 (-52%Z)%Z))%R)%R)%R).
+Theorem var_value4 : forall (x:Z),
+  ((var_as_double x) = (((pow21 52%Z) + (IZR (pow2 31%Z)))%R + (IZR x))%R).
 (* YOU MAY EDIT THE PROOF BELOW *)
 intro.
-unfold var_as_double.
-rewrite double_of_bv64_value.
-rewrite sign_var.
-rewrite sign_value_false.
-rewrite exp_var.
-rewrite mantissa_var.
-rewrite Rmult_1_l.
-auto with *.
-rewrite exp_var.
+rewrite var_value3.
+rewrite distr_pow52.
 auto with *.
 Qed.
 (* DO NOT EDIT BELOW *)
